

## Solution

Let

$$(1 + \sqrt{2})^n = a_n + b_n\sqrt{2} \in \mathbb{Z}(\sqrt{2})$$

Since

$$(\sqrt{2} + 1)^{2026} + (\sqrt{2} - 1)^{2026} = 2a_n, \text{ and } \sqrt{2} - 1 < 1$$

Hence

$$\lfloor (1 + \sqrt{2})^{2026} \rfloor = \lfloor 2a_n - (\sqrt{2} - 1)^{2026} \rfloor = 2a_n - 1$$

There is a recursion relation:

$$\begin{pmatrix} a_{n+1} \\ b_{n+1} \end{pmatrix} = \begin{pmatrix} 1 & 2 \\ 1 & 1 \end{pmatrix} \begin{pmatrix} a_n \\ b_n \end{pmatrix}$$

Consider the vector  $(a_n, b_n)^T \pmod{10}$ :

$$\begin{aligned} (1, 0)^T &\rightarrow (1, 1)^T \\ &\rightarrow (3, 2)^T \\ &\rightarrow (7, 5)^T \\ &\rightarrow (17, 12)^T \equiv (7, 2) \\ &\rightarrow (11, 9) \equiv (1, 9) \\ &\rightarrow (19, 10) \equiv (-1, 0) \end{aligned}$$

So the cycle is of length 12. Let  $\tilde{a}_n := a \pmod{10}$ .

Since  $2026 = 12 \cdot 168 + 10$ ,  $a_{2026} = \tilde{a}_{10} \equiv -7 \equiv 3$ , the answer is  $2 \cdot 3 - 1 = 5$ .